[Parikh] reformulate lemmas

Parikh/Parikh.thy
@@ -3,76 +3,154 @@ theory Parikh
     "../CFG"
     "../CFL"
     "$AFP/Regular-Sets/Regular_Set"
+    "$AFP/Regular-Sets/Regular_Exp"
 begin
 
-sledgehammer_params [provers = cvc4 verit z3 spass vampire zipperposition]
 
-section \<open>regular functions\<close>
+section \<open>functions of languages\<close>
+
+datatype 'a lfun = V nat
+                 | N "'a lang"
+                 | Union2 "'a lfun" "'a lfun"
+                 | UnionC "nat \<Rightarrow> 'a lfun"
+                 | Conc "'a lfun" "'a lfun"
+                 | Star "'a lfun"
+
+type_synonym 'a state = "nat \<Rightarrow> 'a lang"
+
+primrec eval :: "'a lfun \<Rightarrow> 'a state \<Rightarrow> 'a lang" where
+  "eval (V n) s = s n" |
+  "eval (N l) _ = l" |
+  "eval (Union2 f g) s = eval f s \<union> eval g s" |
+  "eval (UnionC f) s = (\<Union>i. eval (f i) s)" |
+  "eval (Conc f g) s = eval f s @@ eval g s" |
+  "eval (Star f) s = star (eval f s)"
+
+primrec vars :: "'a lfun \<Rightarrow> nat set" where
+  "vars (V n) = {n}" |
+  "vars (N _) = {}" |
+  "vars (Union2 f g) = vars f \<union> vars g" |
+  "vars (UnionC f) = (\<Union>i. vars (f i))" |
+  "vars (Conc f g) = vars f \<union> vars g" |
+  "vars (Star f) = vars f"
+
+primrec subst :: "'a lfun \<Rightarrow> (nat \<Rightarrow> 'a lfun) \<Rightarrow> 'a lfun" where
+  "subst (V n) s = s n" |
+  "subst (N l) _ = N l" |
+  "subst (Union2 f g) s = Union2 (subst f s) (subst g s)" |
+  "subst (UnionC f) s = UnionC (\<lambda>i. subst (f i) s)" |
+  "subst (Conc f g) s = Conc (subst f s) (subst g s)" |
+  "subst (Star f) s = Star (subst f s)"
 
 
+section \<open>Regular functions\<close>
+
+inductive regular_fun :: "'a lfun \<Rightarrow> bool" where
+  "regular_fun (V _)" |
+  "regular_lang l \<Longrightarrow> regular_fun (N l)" |
+  "\<lbrakk> regular_fun f; regular_fun g \<rbrakk> \<Longrightarrow> regular_fun (Union2 f g)" |
+  "\<lbrakk> regular_fun f; regular_fun g \<rbrakk> \<Longrightarrow> regular_fun (Conc f g)" |
+  "regular_fun f \<Longrightarrow> regular_fun (Star f)"
+
+lemma regular_fun_regular:
+  assumes "regular_fun f"
+      and "n \<in> vars f \<Longrightarrow> regular_lang (s n)"
+    shows "regular_lang (eval f s)"
+  sorry
+
+lemma regular_fun_mono:
+  assumes "regular_fun f"
+      and "\<forall>i. s i \<subseteq> s' i"
+    shows "eval f s \<subseteq> eval f s'"
+  sorry
+
+
+section \<open>Parikh image\<close>
+
+definition parikh_vec :: "'t list \<Rightarrow> ('t \<Rightarrow> nat)" where
+  "parikh_vec xs c = length (filter (\<lambda>x. c = x) xs)"
+
+definition parikh_img :: "'t lang \<Rightarrow> ('t \<Rightarrow> nat) set" where
+  "parikh_img L = { parikh_vec w | w. w \<in> L }"
+
+(* TODO: really necessary? *)
+definition subseteq_comm :: "'t lang \<Rightarrow> 't lang \<Rightarrow> bool" where
+  "subseteq_comm L1 L2 \<equiv> parikh_img L1 \<subseteq> parikh_img L2"
 
 
 section \<open>systems of equations\<close>
 
-definition "ineq_sat f i xs \<equiv> ((xs ! i) \<supseteq> f i xs)"
-definition "eq_sat f i xs \<equiv> ((xs ! i) = f i xs)"
+type_synonym 'a eq_sys = "'a lfun list"
 
-definition "sat_system_ineq f n xs \<equiv> \<forall>i. (i\<le>n \<longrightarrow> ineq_sat f i xs)"
-definition "sat_system_eq f n xs \<equiv> \<forall>i. (i\<le>n \<longrightarrow> eq_sat f i xs)"
+(* sys independent on variables \<le> n *)
+definition indep :: "'a eq_sys \<Rightarrow> nat \<Rightarrow> bool" where
+  "indep sys n \<equiv> \<forall>eq \<in> set sys. \<forall>x \<in> vars eq. x > n"
 
-locale f_ineq_gs =
-  fixes f :: "nat \<Rightarrow> 'a lang list \<Rightarrow> 'a lang"
+definition solves_ineq_sys :: "'a eq_sys \<Rightarrow> 'a state \<Rightarrow> bool" where
+  "solves_ineq_sys sys s \<equiv> \<forall>i < length sys. eval (sys ! i) s \<subseteq> s i"
+
+definition solves_eq_sys :: "'a eq_sys \<Rightarrow> 'a state \<Rightarrow> bool" where
+  "solves_eq_sys sys s \<equiv> \<forall>i < length sys. eval (sys ! i) s = s i"
+
+definition solves_ineq_sys_comm :: "'a eq_sys \<Rightarrow> 'a state \<Rightarrow> bool" where
+  "solves_ineq_sys_comm sys s \<equiv> \<forall>i < length sys. parikh_img (eval (sys ! i) s) \<subseteq> parikh_img (s i)"
+
+definition solves_eq_sys_comm :: "'a eq_sys \<Rightarrow> 'a state \<Rightarrow> bool" where
+  "solves_eq_sys_comm sys s \<equiv> \<forall>i < length sys. parikh_img (eval (sys ! i) s) = parikh_img (s i)"
+
+definition sys_subst :: "'a eq_sys \<Rightarrow> (nat \<Rightarrow> 'a lfun) \<Rightarrow> 'a eq_sys" where
+  "sys_subst sys s \<equiv> map (\<lambda>eq. subst eq s) sys"
+
+definition partial_sol :: "'a eq_sys \<Rightarrow> 'a eq_sys \<Rightarrow> bool" where
+  "partial_sol sys sol \<equiv> length sol = length sys \<and> indep sol (length sys - 1)
+                  \<and> (\<forall>s. solves_eq_sys_comm (sys_subst sys (\<lambda>i. if i < length sys then sol ! i else V i)) s)"
+
+
+section \<open>Lemma 1\<close>
+
+(* TODO: change this, probably remove locale *)
+locale tmp =
+  fixes f_sys :: "'a eq_sys"
   fixes m :: nat
   fixes r :: nat
-  fixes xs :: "'a lang list"
-  fixes ys :: "'a lang list"
   assumes "r \<le> m"
-  assumes "length xs = r+1"
-  assumes "length ys = m - r"
-  assumes f_regular: "True" (* TODO! *)
+  assumes "length f_sys = r+1"
+  assumes f_regular: "\<forall>eq \<in> set f_sys. regular_fun eq"
 begin
 
-fun comp_xs_aux :: "nat \<Rightarrow> nat \<Rightarrow> 'a lang list" where
-  "comp_xs_aux _ 0 = []"|
-  "comp_xs_aux 0 (Suc i) = {}#(comp_xs_aux 0 i)"|
-  "comp_xs_aux (Suc n) (Suc i) = (f n ((comp_xs_aux n (length xs))@ys))#(comp_xs_aux (Suc n) i)"
+fun g_pre :: "nat \<Rightarrow> nat \<Rightarrow> 'a lfun" where
+  "g_pre _ 0 = N {}" |
+  "g_pre i (Suc n) = subst (f_sys ! i) (\<lambda>j. if j \<le> r then g_pre j n else V j)"
 
-definition "Xs n = comp_xs_aux n (length xs)"
+definition g :: "nat \<Rightarrow> 'a lfun" where
+  "g i \<equiv> UnionC (\<lambda>n. g_pre i n)"
 
-fun g_pre :: "nat \<Rightarrow> nat  \<Rightarrow> 'a lang" where
-  "g_pre i 0  = {}"|
-  "g_pre i (Suc n) = f i ((Xs n)@ys)"
-
-lemma g_pre_index: "i < length xs \<Longrightarrow> g_pre i n = (comp_xs_aux n i) ! i "
+(* The lemma from the paper *)
+lemma lemma1: "\<exists>g_sys. length g_sys = r+1 \<and> indep g_sys r
+                \<and> (solves_ineq_sys f_sys s \<longrightarrow> solves_ineq_sys g_sys s)
+                \<and> (solves_eq_sys g_sys s \<longrightarrow> solves_eq_sys f_sys s)"
   sorry
 
-definition "g i \<equiv> \<Union>n. g_pre i n"
+(* TODO: really necessary *)
+definition eq_sys_subseteq :: "'a eq_sys \<Rightarrow> 'a eq_sys \<Rightarrow> bool" where
+  "eq_sys_subseteq gs gs' \<equiv> (\<forall>s. \<forall>i\<le>r. subseteq_comm (eval (gs ! i) s) (eval (gs' ! i) s))"
 
-lemma "g_pre i (Suc n) \<subseteq> f i (xs @ ys)"
-proof
-  fix x
-  assume "x \<in> g_pre i (Suc n)"
-  then have "x \<in> f i ((Xs n)@ys)" by auto
-  show "x \<in> f i (xs@ys)" sorry
-qed
-  
+lemma lemma2_aux:
+  assumes "regular_fun f0"
+  shows "\<exists>g0. regular_fun g0 \<and> partial_sol [f0] [g0]
+            \<and> (\<forall>g0'. partial_sol [f0] [g0'] \<longrightarrow>
+                (\<forall>s. parikh_img (eval g0 s) \<subseteq> parikh_img (eval g0' s)))"
+  sorry
 
-lemma lemma1_aux_1:
-  assumes f_sub: "\<forall>i\<le>r. (xs ! i) \<supseteq> f i (xs@ys)"
-  shows "\<forall>i\<le>r. (xs ! i) \<supseteq> g i"
-proof
-  fix i
-  show "i \<le> r \<longrightarrow> g i \<subseteq> xs ! i"
-    proof
-      assume "i\<le>r"
-      with f_sub have "f i (xs @ ys) \<subseteq> xs ! i" by simp
-      show "g i \<subseteq> xs ! i" sorry
-    qed
-qed
-  
-lemma lemma1:
-  "\<exists>g. ((\<forall>i. (i\<le>r \<longrightarrow> (xs ! i) \<supseteq> f i (xs@ys))) \<longrightarrow> (\<forall>i. (i\<le>r \<longrightarrow> (xs ! i) \<supseteq> g i ys))) \<and>
-       ((\<forall>i. (i\<le>r \<longrightarrow> (xs ! i) = g i ys)) \<longrightarrow> (\<forall>i. (i\<le>r \<longrightarrow> (xs ! i) = f i (xs @ ys))))"
+(* The theorem from the paper *)
+lemma lemma2: "\<exists>gs. (\<forall>g \<in> set gs. regular_fun g) \<and> partial_sol f_sys gs
+                  \<and> (\<forall>gs'. partial_sol f_sys gs' \<longrightarrow> eq_sys_subseteq gs gs')"
+  sorry
+
+lemma
+  assumes "r = m"
+  shows "\<exists>s. (\<forall>i. regular_lang (s i)) \<and> solves_eq_sys_comm f_sys s
+          \<and> (\<forall>s'. solves_eq_sys_comm f_sys s' \<longrightarrow> (\<forall>i. parikh_img (s' i) \<subseteq> parikh_img (s i)))"
   sorry
 
 end
